some progress for incoming fragments in TLS; some HS support needed to integrate with client/server tests

src/tls/Handshake.fst
@@ -1,22 +1,105 @@
 ﻿(* Copyright (C) 2012--2015 Microsoft Research and INRIA *)
 
-#light "off"
-
-(* Handshake protocol messages *)
 module Handshake
-open TLSExtensions //the other opens are in the .fsti
-open CoreCrypto
+
+open FStar.Heap
+open FStar.HyperHeap
+//FIXME! Don't open so much ... gets confusing. Use module abbrevs instead
+open FStar.Seq
+open FStar.SeqProperties // for e.g. found
+open FStar.Set  
+
+open Platform.Error
+open Platform.Bytes
+
+open TLSError
+open TLSInfo
+open TLSConstants
+open Range
+open HandshakeMessages
 open HSCrypto
+open StAE
+
+//16-05-31 these opens are implementation-only; overall we should open less
+open TLSExtensions 
+open CoreCrypto
 open HandshakeLog
 
-let hsId h = noId // Placeholder
 
+module HH = FStar.HyperHeap
+module MR = FStar.Monotonic.RRef
+module MS = MonotoneSeq
+
+#set-options "--lax" 
+
+// represents the outcome of a successful handshake, 
+// providing context for the derived epoch
+type handshake = 
+  | Fresh of sessionInfo
+  | Resumed of abbrInfo * sessionInfo //changed: was hs * seq epoch (creating cycle)
+// We use SessionInfo as unique session indexes.
+// We tried using instead hs, but this creates circularities
+// We'll probably need a global log to reason about them.
+// We should probably do the same in the session store.
+
+// extracts a transport key identifier from a handshake record
+val hsId: handshake -> Tot id 
+//16-05-31 TODO breaking TC in TLS; was (i:id { is_stream_ae i }) //16-05-19 focus on TLS 1.3
+
+let hsId h = noId // Placeholder 
+
+
+//<expose for TestClient>
 (* Negotiation: HELLO sub-module *)
+private type ri = cVerifyData * sVerifyData 
+type b_log = bytes 
 
-let ri = (cVerifyData * sVerifyData) 
+
+type eph_s = option kex_s_priv
+type eph_c = list kex_s_priv
+type nego = {
+     n_resume: bool;
+     n_client_random: TLSInfo.random;
+     n_server_random: TLSInfo.random;
+     n_sessionID: option sessionID;
+     n_protocol_version: protocolVersion;
+     n_kexAlg: TLSConstants.kexAlg;
+     n_aeAlg: TLSConstants.aeAlg;
+     n_sigAlg: option TLSConstants.sigAlg;
+     n_cipher_suite: cipherSuite;
+     n_dh_group: option namedGroup;
+     n_compression: option compression;
+     n_extensions: negotiatedExtensions;
+     n_scsv: list scsv_suite;
+}                 
+
+type hs_id = {
+     id_cert: Cert.chain;
+     id_sigalg: option sigHashAlg;
+}
+
+type session = {
+     session_nego: nego;
+}     
 
 
+val getId: KeySchedule.recordInstance -> GTot id
+let getId k = 
+    match k with
+    | KeySchedule.StAEInstance #i rd wr -> i
+    | KeySchedule.StLHAEInstance #i rd wr -> i
 
+val recordInstanceToEpoch: h:handshake -> ks:KeySchedule.recordInstance -> (StAE.reader (peerId (hsId h)) * StAE.writer (hsId h))
+let recordInstanceToEpoch hs ri = 
+    match ri with
+    | KeySchedule.StAEInstance #i rd wr -> (StAE.Stream () rd),(StAE.Stream () wr)
+    | KeySchedule.StLHAEInstance #i rd wr -> (StAE.StLHAE () rd),(StAE.StLHAE () wr)
+       
+    
+
+val prepareClientHello: config -> KeySchedule.ks -> HandshakeLog.log -> option ri -> option sessionID -> ST (hs_msg * bytes)
+  (requires (fun h -> True))
+  (ensures (fun h0 i h1 -> True))
 let prepareClientHello cfg ks log ri sido =
   let cr = KeySchedule.ks_client_random ks in
   let kp = 
@@ -86,6 +169,9 @@ let rec negotiateGroupKeyShare cfg pv kex exts =
     
 
 // FIXME: TLS1.3
+val prepareServerHello: config -> KeySchedule.ks -> HandshakeLog.log -> option ri -> (hs_msg * bytes) -> ST (result (nego * option KeySchedule.recordInstance * (hs_msg * bytes)))
+  (requires (fun h -> True))
+  (ensures (fun h0 i h1 -> True))
 let prepareServerHello cfg ks log ri (ClientHello ch,_) =
   match negotiateVersion cfg ch.ch_protocol_version with
     | Error(z) -> Error(z)
@@ -134,7 +220,13 @@ let prepareServerHello cfg ks log ri (ClientHello ch,_) =
        n_resume = false} in
     let _ = log @@ (ClientHello ch) in
     let shb = log @@ (ServerHello sh) in
-    Correct (nego,(ServerHello sh,shb))
+    let lb = HandshakeLog.getHash log in
+    let keys = (match pv with
+    	     | TLS_1p3 -> 
+	       let keys = KeySchedule.ks_server_13_get_htk ks lb  in
+	       Some keys
+	     | _ -> None) in
+    Correct (nego,keys,(ServerHello sh,shb))
 
 (* Is this one of the special random values indicated by the RFC (6.3.1.1)? *)
 val isSentinelRandomValue: protocolVersion -> protocolVersion -> TLSInfo.random -> Tot bool
@@ -169,6 +261,10 @@ let acceptableCipherSuite cfg ch s_pv s_cs =
   List.Tot.existsb (fun x -> x = s_cs) cfg.ciphersuites &&
   not (isAnonCipherSuite s_cs) || cfg.allowAnonCipherSuite
   
+val processServerHello: c:config -> KeySchedule.ks -> HandshakeLog.log -> option ri -> ch -> (hs_msg * bytes) ->
+                        ST (result (nego * option KeySchedule.recordInstance))
+  (requires (fun h -> True))
+  (ensures (fun h0 i h1 -> True))
 let processServerHello cfg ks log ri ch (ServerHello sh,_) =
   let _ = log @@ (ServerHello sh) in
   // Assuming no resumption; TODO: add it 
@@ -259,11 +355,206 @@ type handshake_state' (r:role) =
      }
 
 //NS: needed this renaming trick for the .fsti
+//16-05-31 this type should be private to HS
 let handshake_state r = handshake_state' r
+
+let resume_id (r:role) = o:option sessionID{r=Server ==> o=None}
+
+
+//</expose for TestClient>
+
+// relocate?
+type fresh_subregion r0 r h0 h1 = fresh_region r h0 h1 /\ extends r r0
+
+type epoch_region_inv (#i:id) (hs_rgn:rgn) (r:reader (peerId i)) (w:writer i) =
+  disjoint hs_rgn (region w)                  /\
+  parent (region w) <> FStar.HyperHeap.root    /\
+  parent (region r) <> FStar.HyperHeap.root    /\
+  parent hs_rgn = parent (parent (region w))  /\ //Grandparent of each writer is a sibling of the handshake
+  disjoint (region w) (region r)              /\
+  is_epoch_rgn (region w)                     /\ //they're all colored as epoch regions
+  is_epoch_rgn (region r)                     /\
+  is_epoch_rgn (parent (region w))            /\
+  is_epoch_rgn (parent (region r))            /\
+  is_hs_rgn hs_rgn                              //except for the hs_rgn, of course
+
+abstract type epoch_region_inv' (#i:id) (hs_rgn:rgn) (r:reader (peerId i)) (w:writer i) =
+  epoch_region_inv hs_rgn r w
+  
+module I = IdNonce
+
+type epoch (hs_rgn:rgn) (n:TLSInfo.random) = 
+  | Epoch: h: handshake ->
+           r: reader (peerId (hsId h)) ->
+           w: writer (hsId h) {epoch_region_inv' hs_rgn r w /\ I.nonce_of_id (hsId h) = n} 
+	   -> epoch hs_rgn n
+  // we would extend/adapt it for TLS 1.3,
+  // e.g. to notify 0RTT/forwad-privacy transitions
+  // for now epoch completion is a total function on handshake --- should be stateful
+
+let reveal_epoch_region_inv_all (u:unit)
+  : Lemma (forall i hs_rgn r w.{:pattern (epoch_region_inv' #i hs_rgn r w)}
+	   epoch_region_inv' #i hs_rgn r w
+	   <==>
+   	   epoch_region_inv #i hs_rgn r w)
+  = ()	   
+
+let reveal_epoch_region_inv (#hs_rgn:rgn) (#n:TLSInfo.random) (e:epoch hs_rgn n) 
+  : Lemma (let r = Epoch.r e in 
+	   let w = Epoch.w e in 
+	   epoch_region_inv hs_rgn r w)
+  = ()
+
+let writer_epoch (#hs_rgn:rgn) (#n:TLSInfo.random) (e:epoch hs_rgn n) 
+  : Tot (w:writer (hsId (e.h)) {epoch_region_inv hs_rgn (Epoch.r e) w})
+  = Epoch.w e
+
+let reader_epoch (#hs_rgn:rgn) (#n:TLSInfo.random) (e:epoch hs_rgn n) 
+  : Tot (r:reader (peerId (hsId (e.h))) {epoch_region_inv hs_rgn r (Epoch.w e)})
+  = match e with | Epoch h r w -> r //16-05-20 Epoch.r e failed.
+
+(* The footprint just includes the writer regions *)
+abstract let epochs_inv (#r:rgn) (#n:TLSInfo.random) (es: seq (epoch r n)) =
+  forall (i:nat { i < Seq.length es })
+    (j:nat { j < Seq.length es /\ i <> j}).{:pattern (Seq.index es i); (Seq.index es j)}
+    let ei = Seq.index es i in
+    let ej = Seq.index es j in
+    parent (region ei.w) = parent (region ej.w) /\  //they all descend from a common epochs sub-region of the connection
+    disjoint (region ei.w) (region ej.w)           //each epoch writer lives in a region disjoint from the others
+
+abstract let epochs_inv' (#r:rgn) (#n:TLSInfo.random) (es: seq (epoch r n)) = epochs_inv es
+
+let epochs (r:rgn) (n:TLSInfo.random) = es: seq (epoch r n) { epochs_inv' es }
+
+let reveal_epochs_inv' (u:unit)
+  : Lemma (forall (r:rgn) (#n:TLSInfo.random) (es:seq (epoch r n)). {:pattern (epochs_inv' es)}
+	     epochs_inv' es
+	     <==>
+	     epochs_inv es)
+  = ()
+
+// internal stuff: state machine, reader/writer counters, etc.
+// (will take other HS fields as parameters)
+
+type hs =
+  | HS: #region: rgn { is_hs_rgn region } ->
+              r: role ->
+         resume: resume_id r ->
+            cfg: config ->
+          nonce: TLSInfo.random ->  // unique for all honest instances; locally enforced; proof from global HS invariant? 
+            log: MS.i_seq region (epoch region nonce) epochs_inv ->  // append-only, monotonic log of epochs
+          state: rref region (handshake_state r)  ->       // opaque, subject to invariant
+             hs
+
+
+(* the handshake internally maintains epoch 
+   indexes for the current reader and writer *)
+
+let logT (s:hs) (h:HyperHeap.t) = MS.i_sel h s.log
+
+let stateType (s:hs) = epochs s.region s.nonce * handshake_state (HS.r s)
+
+let stateT (s:hs) (h:HyperHeap.t) : stateType s = (logT s h, sel h s.state)
+
+let non_empty h s = Seq.length (logT s h) > 0
+
+let logIndex (#t:Type) (log: seq t) = n:int { -1 <= n /\ n < Seq.length log }
+
+let forall_epochs (hs:hs) h (p:(epoch hs.region hs.nonce -> Type)) = 
+  (let es = logT hs h in
+   forall (i:nat{i < Seq.length es}).{:pattern (Seq.index es i)} p (Seq.index es i))
+     
+(* //vs modifies clauses? *)
+(* let unmodified_epochs s h0 h1 =  *)
+(*   forall_epochs s h0 (fun e ->  *)
+(*     let rs = regions e in  *)
+(*     (forall (r:rid{Set.mem r rs}).{:pattern (Set.mem r rs)} Map.sel h0 r = Map.sel h1 r)) *)
+
+//epochs in h1 extends epochs in h0 by one 
+let fresh_epoch h0 s h1 =
+  let es0 = logT s h0 in 
+  let es1 = logT s h1 in 
+  Seq.length es1 > 0 &&
+  es0 = Seq.slice es1 0 (Seq.length es1 - 1)
+
+let latest h (s:hs{Seq.length (logT s h) > 0}) = // accessing the latest epoch
+ let es = logT s h in
+ Seq.index es (Seq.length es - 1)
+
+// separation policy: the handshake mutates its private state, 
+// only depends on it, and only extends the log with fresh epochs.
+
+
+// placeholder, to be implemented as a stateful property.
+assume val completed: #region:rgn -> #nonce:TLSInfo.random -> epoch region nonce -> Type0
+
+// consider adding an optional (resume: option sid) on the client side
+// for now this bit is not explicitly authenticated.
+
+// Well-formed logs are all prefixes of (Epoch; Complete)*; Error
+// This crucially assumes that TLS keeps track of OutCCS and InCCSAck
+// so that it knows which reader & writer to use (not always the latest ones):
+// - within InCCSAck..OutCCS, we still use the older writer
+// - within OutCCS..InCCSAck, we still use the older reader
+// - otherwise we use the latest readers and writers
+
+// technicality: module dependencies?
+// we used to pre-declare all identifiers in TLSInfo
+// we used owe could also record (fatal) errors as log terminators
+ 
+// abstract invariant; depending only on the HS state (not the epochs state)
+// no need for an epoch states invariant here: the HS never modifies them
+ 
+assume val hs_invT : s:hs -> epochs:seq (epoch s.region s.nonce) -> handshake_state (HS.r s) -> Type0
+
+let hs_inv (s:hs) (h: HyperHeap.t) = 
+  hs_invT s (logT s h) (sel h (HS.state s))  //An abstract invariant of HS-internal state
+  /\ MS.i_contains s.log h                    //Nothing deep about these next two, since they can always 
+  /\ HyperHeap.contains_ref s.state h                 //be recovered by 'recall'; carrying them in the invariant saves the trouble
+
 
 //to match the external interface
 //let handshake_state (r:role) = handshake_state' r
+val iT0: s:hs -> rw:rw -> st:stateType s -> Tot (logIndex (fst st))
 let iT0 s rw st = -1 //TODO:Implement!
+// returns the current index in the log for reading or writing, or -1 if there is none.
+// depends only on the internal state of the handshake
+let iT s rw h = iT0 s rw (stateT s h) 
+
+//A framing lemma with a very trivial proof, because of the way stateT abstracts the state-dependent parts
+let frame_iT_trivial  (s:hs) (rw:rw) (h0:HH.t) (h1:HH.t) 
+  : Lemma (stateT s h0 = stateT s h1
+           ==> iT s rw h0 = iT s rw h1) 
+  = ()	                               
+
+//Here's a framing on stateT connecting it to the region discipline
+let frame_stateT  (s:hs) (rw:rw) (h0:HH.t) (h1:HH.t) (mods:Set.set rid)
+  : Lemma (requires HH.modifies_just mods h0 h1
+		    /\ Map.contains h0 s.region
+		    /\ not (Set.mem s.region mods))
+          (ensures stateT s h0 = stateT s h1)
+  = ()	                               
+
+//This is probably the framing lemma that a client of this module will want to use
+let frame_iT  (s:hs) (rw:rw) (h0:HH.t) (h1:HH.t) (mods:Set.set rid)
+  : Lemma (requires HH.modifies_just mods h0 h1
+		    /\ Map.contains h0 s.region
+		    /\ not (Set.mem s.region mods))
+          (ensures stateT s h0 = stateT s h1
+		   /\ iT s rw h0 = iT s rw h1)
+  = frame_stateT s rw h0 h1 mods;
+    frame_iT_trivial s rw h0 h1
+    
+// returns the epoch for reading or writing
+let eT s rw (h:HyperHeap.t { iT s rw h >= 0 }) = Seq.index (logT s h) (iT s rw h)
+
+let readerT s h = eT s Reader h 
+let writerT s h = eT s Writer h
+
+// this function increases (how to specify it once for all?)
+val i: s:hs -> rw:rw -> ST int 
+  (requires (fun h -> True))
+  (ensures (fun h0 i h1 -> h0 = h1 /\ i = iT s rw h1))
 let i s rw = Platform.Error.unexpected "i: not yet implemented" //TODO:Implement
 
 val handshake_state_init: (cfg:TLSInfo.config) -> (r:role) -> (reg:rid) -> ST (handshake_state r)
@@ -282,18 +573,35 @@ let handshake_state_init cfg (r:role) (reg:rid) =
     	| Client -> C (C_Idle None)
     	| Server -> S (S_Idle None)) }
 
-//Defined in the .fsti
-//type handshake
-//type epoch 
-//type epochs
-//type hs
-//type outgoing
-//type incoming
+// payload of a handshake fragment, to be made opaque eventually
+type message (i:id) = (| rg: frange i & rbytes rg |)
+let out_msg i rg b : message i= (|rg, b|)
 
-(* This following function needs to call PRF.deriveKeys correctly to get StatefulLHAE keys *)
-assume val deriveEpoch: (r:rid) -> (n:TLSInfo.random) -> session -> ST (epoch r n)
-  (requires (fun h -> True))
-  (ensures (fun h0 i h1 -> True))
+// What the HS asks the record layer to do, in that order.
+type outgoing (i:id) (* initial index *) = 
+  | Outgoing: 
+      send_first: option (message i) -> // HS fragment to be sent;  (with current id)
+      send_ccs  : bool               -> // CCS fragment to be sent; (with current id)
+      next_keys : bool               -> // the writer index increases;
+      complete  : bool               -> // the handshake is complete!
+      outgoing i 
+  | OutError: error -> outgoing i       // usage? in case something goes wrong when preparing messages. 
+
+let out_next_keys (#i:id) (r:outgoing i) = is_Outgoing r && Outgoing.next_keys r
+let out_complete (#i:id) (r:outgoing i)  = is_Outgoing r && Outgoing.complete r
+
+type incoming = 
+  // the fragment is accepted, and...
+  | InAck: 
+      next_keys : bool -> // the reader index increases;
+      complete  : bool -> // the handshake is complete!
+      incoming
+
+  | InQuery: Cert.chain -> bool -> incoming // could be part of InAck if no explicit user auth
+  | InError: error -> incoming // how underspecified should it be?
+
+let in_next_keys (r:incoming) = is_InAck r && InAck.next_keys r
+let in_complete (r:incoming)  = is_InAck r && InAck.complete r
 
 (* Handshake API: INTERNAL Callbacks, hidden from API *)
 
@@ -308,7 +616,8 @@ let client_send_client_hello (HS #r0 r res cfg id lgref hsref) =
             hs_buffers = {(!hsref).hs_buffers with hs_outgoing = chb};
 	    hs_state = C(C_HelloSent ri ch)}
   
-	    
+	  
+  
 val client_handle_server_hello: hs -> list (hs_msg * bytes) -> ST incoming
   (requires (fun h -> True))
   (ensures (fun h0 i h1 -> True))
@@ -321,9 +630,13 @@ let client_handle_server_hello (HS #r0 r res cfg id lgref hsref) msgs =
       hsref := {!hsref with
 	       hs_nego = Some n;
 	       hs_state = C(C_HelloReceived n)};
-      InAck)
+      InAck false false)
 
 
+val processServerHelloDone: cfg:config -> nego:nego -> ks:KeySchedule.ks -> log:HandshakeLog.log ->
+    			    list (hs_msg*bytes) -> list (hs_msg * bytes) -> ST (result (list (hs_msg * bytes)))
+  (requires (fun h -> nego.n_protocol_version <> TLS_1p3))
+  (ensures (fun h0 i h1 -> True))
 let processServerHelloDone cfg n ks log msgs opt_msgs =
   match msgs with
   | [(Certificate(c),_); (ServerKeyExchange(ske),_); (ServerHelloDone,_)] when 
@@ -362,11 +675,11 @@ let processServerHelloDone cfg n ks log msgs opt_msgs =
 	      let _ = log @@ ServerKeyExchange(ske) in
 	      let _ = log @@ CertificateRequest(cr) in
 	      let _ = log @@ ServerHelloDone in
-	      let b1 = log @@ ClientKeyExchange cke in	
+	      let b1 = log @@ Certificate(cc) in
+	      let b2 = log @@ ClientKeyExchange cke in	
 	      let lb = HandshakeLog.getBytes log in
 	      if ems then KeySchedule.ks_client_12_set_session_hash ks lb;
-	      let b2 = log @@ Certificate(cc) in
-      	    Correct [ClientKeyExchange cke,b1; Certificate cc,b2])
+      	    Correct [(Certificate cc,b1); (ClientKeyExchange cke,b2)])
 	  | _ -> Error (AD_handshake_failure, perror __SOURCE_FILE__ __LINE__ "only support ECDHE/DHE SKE")
          )
        // Signature verification failed
@@ -388,15 +701,18 @@ let client_handle_server_hello_done (HS #r0 r res cfg id lgref hsref) msgs opt_m
              hsref := {!hsref with 
                 hs_buffers = {(!hsref).hs_buffers with hs_outgoing = b1};
                 hs_state = C(C_OutCCS n)};
-              InAck
+              InAck false false
       | Correct [(ClientKeyExchange(cke),b1);(Certificate(cc),b2)] ->
              hsref := {!hsref with 
                 hs_buffers = {(!hsref).hs_buffers with hs_outgoing = b1 @| b2};
                 hs_state = C(C_OutCCS n)};
-              InAck
+              InAck false false
       | Error (x,y) -> InError(x,y))
    | _ -> InError (AD_handshake_failure, perror __SOURCE_FILE__ __LINE__ "unexpected state")
 
+val prepareClientFinished: KeySchedule.ks -> HandshakeLog.log -> ST (hs_msg * bytes)
+  (requires (fun h -> True))
+  (ensures (fun h0 i h1 -> True))
 let prepareClientFinished ks log = 
     let lb = HandshakeLog.getBytes log in
     let fin = {fin_vd = KeySchedule.ks_client_12_client_verify_data ks lb} in
@@ -425,8 +741,11 @@ let client_handle_server_ccs (HS #r0 r res cfg id lgref hsref) msgs =
       let _ = (!hsref).hs_log @@ SessionTicket(stick) in
       hsref := {!hsref with
 	       hs_state = C(C_CCSReceived n vd)};
-      InAck
+      InAck false false
 
+val processServerFinished: KeySchedule.ks -> HandshakeLog.log -> (hs_msg * bytes) -> ST (result bytes)
+  (requires (fun h -> True))
+  (ensures (fun h0 i h1 -> True))
 let processServerFinished ks log (m,l) =
    match m with
    | Finished(f) ->
@@ -449,9 +768,13 @@ let client_handle_server_finished (HS #r0 r res cfg id lgref hsref) msgs =
     | Correct svd -> 
        hsref := {!hsref with
   		 hs_state = C(C_Idle (Some (vd,svd)))};
-       InAck)
+       InAck false false)
     
 
+val processServerFinished_13: cfg:config -> n:nego -> ks:KeySchedule.ks -> log:HandshakeLog.log ->
+    			      list (hs_msg*bytes) -> ST (result (list (hs_msg * bytes) * bytes * KeySchedule.recordInstance))
+  (requires (fun h -> True))
+  (ensures (fun h0 i h1 -> True))
 let processServerFinished_13 cfg n ks log msgs =
    let rem,creq = 
      match msgs with
@@ -506,12 +829,12 @@ let client_handle_server_finished_13 (HS #r0 r res cfg id lgref hsref) msgs =
        hsref := {!hsref with
                  hs_buffers = {(!hsref).hs_buffers with hs_outgoing = fb};
   		 hs_state = C(C_Idle (Some (vd,svd)))};
-       InAck
+       InAck false false
     | Correct ([(Certificate c,cb);(Finished f,fb)],svd,keys) -> 
        hsref := {!hsref with
                  hs_buffers = {(!hsref).hs_buffers with hs_outgoing = cb @| fb};
   		 hs_state = C(C_Idle (Some (vd,svd)))};
-       InAck)
+       InAck false false)
     
 
 
@@ -524,13 +847,51 @@ let server_handle_client_hello (HS #r0 r res cfg id lgref hsref) msgs =
   | S(S_Idle ri),[(ClientHello(ch),l)] ->
     (match (prepareServerHello cfg (!hsref).hs_ks (!hsref).hs_log ri (ClientHello ch,l)) with
      | Error z -> InError z
-     | Correct (n,(sh,shb)) ->
+     | Correct (n,keys,(sh,shb)) ->
        hsref := {!hsref with
                hs_buffers = {(!hsref).hs_buffers with hs_outgoing = shb};
 	       hs_nego = Some n;
 	       hs_state = S(S_HelloSent n)};
-       InAck)
+       InAck false false)
     
+
+let prepareServerHelloDone cfg n ks log = 
+    if (n.n_protocol_version <> TLS_1p3 && is_Some n.n_sigAlg &&
+       (n.n_kexAlg = Kex_DHE || n.n_kexAlg = Kex_ECDHE)) 
+    then 
+    match Cert.lookup_server_chain cfg.cert_chain_file cfg.private_key_file n.n_protocol_version n.n_sigAlg n.n_extensions.ne_signature_algorithms with
+    | Correct (chain, csk) -> 
+      let c = {crt_chain = chain} in
+      let cb = log @@ Certificate(c) in
+      let cr = n.n_client_random in
+      let ems = n.n_extensions.ne_extended_ms in
+      let pv = n.n_protocol_version in 
+      let cs = n.n_cipher_suite in
+      let Some gn = n.n_dh_group in
+      let gy = KeySchedule.ks_server_12_init_dh ks cr pv cs ems gn in
+
+      let kex_s = KEX_S_DHE gy in
+      let sv = kex_s_to_bytes kex_s in
+      let csr = n.n_client_random @| n.n_server_random in
+
+      // Signature agility (following the broken rules of 7.4.1.4.1. in RFC5246)
+      let Some sa = n.n_sigAlg in
+      let algs = match n.n_extensions.ne_signature_algorithms with
+        | None -> [sa,Hash CoreCrypto.SHA1] | Some l -> l in
+      let algs = List.Tot.filter (fun (s,_)->s=sa) algs in
+      let alg = match algs with | h::_ -> h | [] -> (sa, Hash CoreCrypto.SHA1) in
+      (match Cert.sign pv Server (Some csr) csk alg sv with
+      | Correct signature -> 
+         let ske = {ske_kex_s = kex_s; ske_sig = signature} in
+         let skeb = log @@ ServerKeyExchange(ske) in
+         let shdb = log @@ ServerHelloDone in
+	 Correct [(Certificate(c),cb);(ServerKeyExchange(ske),skeb);(ServerHelloDone,shdb)]
+      | Error z -> Error z)
+    | Error z -> Error z
+    else 
+       Error (AD_handshake_failure, perror __SOURCE_FILE__ __LINE__ "should not call this function in TLS 1.3")
+
+ 
 
 val server_send_server_hello_done: hs -> ST unit
   (requires (fun h -> True))
@@ -540,73 +901,204 @@ let server_send_server_hello_done (HS #r0 r res cfg id lgref hsref) =
   | S(S_HelloSent n) 
     when (n.n_protocol_version <> TLS_1p3 &&
 	 (n.n_kexAlg = Kex_DHE || n.n_kexAlg = Kex_ECDHE)) ->
-    (match Cert.lookup_server_chain cfg.cert_chain_file cfg.private_key_file n.n_protocol_version n.n_sigAlg n.n_extensions.ne_signature_algorithms with
-    | Correct (chain, csk) -> 
-      let c = {crt_chain = chain} in
-      let cb = certificateBytes n.n_protocol_version c in
-      let gy = CommonDH.keygen CommonDH.default_group in
-      let kex_s = KEX_S_DHE gy in
-      let sv = kex_s_to_bytes kex_s in
-      let csr = n.n_client_random @| n.n_server_random in
-
-      // Signature agility (following the broken rules of 7.4.1.4.1. in RFC5246
-      let Some sa = n.n_sigAlg in
-      let algs = match n.n_extensions.ne_signature_algorithms with
-        | None -> [sa,Hash CoreCrypto.SHA1] | Some l -> l in
-      let algs = List.Tot.filter (fun (s,_)->s=sa) algs in
-      let alg = match algs with | h::_ -> h | [] -> (sa, Hash CoreCrypto.SHA1) in
-      (match Cert.sign n.n_protocol_version Server (Some csr) csk alg sv with
-      | Correct signature -> 
-         let ske = {ske_kex_s = kex_s; ske_sig = signature} in
-         let skeb = serverKeyExchangeBytes ske in
-         let shd = serverHelloDoneBytes in
-         let nl = cb @| skeb @| shd in
+    (match prepareServerHelloDone cfg n (!hsref).hs_ks (!hsref).hs_log with
+     | Correct ([(Certificate(c),cb);(ServerKeyExchange(ske),skeb);(ServerHelloDone,shdb)]) ->    
+         let nl = cb @| skeb @| shdb in
 	    hsref := {!hsref with
 		 hs_buffers = {(!hsref).hs_buffers with hs_outgoing = nl};
-		 hs_log = (!hsref).hs_log (* @| nl *);
 		 hs_state = S(S_HelloDone n)}
       | Error e -> 
 	  hsref := {!hsref with hs_state = S(S_Error e)})
-    | Error e ->
-        hsref := {!hsref with hs_state = S(S_Error e)})
 
-assume val server_handle_client_ccs: hs -> list (hs_msg * bytes) -> list (hs_msg * bytes) -> ST incoming
+let processClientCCS n ks log msgs opt_msgs = 
+    let rem = 
+    match opt_msgs with
+    | [(Certificate c,_)] ->
+      let _ = log @@ Certificate(c) in
+      Correct msgs
+    | [] -> Correct msgs 
+    | _ -> Error(AD_decode_error, perror __SOURCE_FILE__ __LINE__ "Expected Certificate only before CKE") in
+    match rem with
+    | Correct [(ClientKeyExchange cke,_)] ->
+      let ems = n.n_extensions.ne_extended_ms in
+      let _ = log @@ ClientKeyExchange(cke) in
+      let lb = HandshakeLog.getBytes log in
+      (match cke.cke_kex_c with 
+       | KEX_C_DHE b 
+       | KEX_C_ECDHE b -> 
+             (KeySchedule.ks_server_12_cke_dh ks b lb;
+	      Correct ())
+       | _ -> Error(AD_decode_error, perror __SOURCE_FILE__ __LINE__ "Expected DHE/ECDHE CKE"))
+    | Error z -> Error z
+
+val server_handle_client_ccs: hs -> list (hs_msg * bytes) -> list (hs_msg * bytes) -> ST incoming
   (requires (fun h -> True))
   (ensures (fun h0 i h1 -> True))
 
-(*
-let server_handle_client_ccs (HS #r0 r res cfg id lgref hsref)  msgs opt_msgs = 
-  match (!hsref).hs_state, msgs with
-  | S(S_HelloDone n),[(ClientKeyExchange(cke),l)] when 
+let server_handle_client_ccs (HS #r0 r res cfg id lgref hsref) msgs opt_msgs = 
+  match (!hsref).hs_state with
+  | S(S_HelloDone n) when
      (n.n_protocol_version <> TLS_1p3 && 
       (n.n_kexAlg = Kex_DHE || n.n_kexAlg = Kex_ECDHE)) ->
-      let pms = CommonDH.dh_initiator k 
-*)
+     (match processClientCCS n (!hsref).hs_ks (!hsref).hs_log msgs opt_msgs with
+      | Correct () ->       
+        (hsref := {!hsref with
+	       hs_state = S(S_CCSReceived n)};
+         InAck false false)
+      | Error z -> InError z)
+  
 
-    
-assume val server_handle_client_finished: hs -> list (hs_msg * bytes) -> ST incoming
-  (requires (fun h -> True))
-  (ensures (fun h0 i h1 -> True))
-assume val server_send_server_finished: hs -> ST unit
+let processClientFinished n ks log msgs =   
+    match msgs with
+    | [(Finished f,_)] ->
+      let lb = HandshakeLog.getBytes log in
+      let cvd = KeySchedule.ks_server_12_client_verify_data ks lb in
+      let _ = log @@ Finished(f) in
+      let lb = HandshakeLog.getBytes log in
+      let svd = KeySchedule.ks_server_12_server_verify_data ks lb in
+      let fin = Finished ({fin_vd = svd}) in
+      let finb = log @@ fin in
+      Correct [(fin,finb)]
+   | _ -> Error (AD_unexpected_message, perror __SOURCE_FILE__ __LINE__ "ClientFinished expected")
+
+val server_handle_client_finished: hs -> list (hs_msg * bytes) -> ST incoming
   (requires (fun h -> True))
   (ensures (fun h0 i h1 -> True))
 
+let server_handle_client_finished (HS #r0 r res cfg id lgref hsref) msgs =
+  match (!hsref).hs_state with
+  | S(S_CCSReceived n) -> 
+    match processClientFinished n (!hsref).hs_ks (!hsref).hs_log msgs with
+    | Correct [(Finished(f),finb)] -> 
+        (hsref := {!hsref with
+	       	   hs_buffers = {(!hsref).hs_buffers with hs_outgoing = finb};
+	           hs_state = S(S_OutCCS n)};
+         InAck false false)
+    | Error e -> InError e
 
-assume val server_handle_client_finished_13: hs -> list (hs_msg * bytes) -> list (hs_msg * bytes) -> ST incoming
+val server_send_server_finished: hs -> ST unit
   (requires (fun h -> True))
   (ensures (fun h0 i h1 -> True))
-assume val server_send_server_finished_13: hs -> ST unit
+let server_send_server_finished (HS #r0 r res cfg id lgref hsref) =
+  match (!hsref).hs_state with
+  | S(S_OutCCS n) -> 
+    hsref := {!hsref with
+	       hs_state = S(S_FinishedSent n)}
+
+
+
+
+let prepareServerFinished_13 cfg n ks log = 
+    if (n.n_protocol_version = TLS_1p3 && is_Some n.n_sigAlg &&
+       (n.n_kexAlg = Kex_DHE || n.n_kexAlg = Kex_ECDHE))
+    then 
+    let ee = {ee_extensions = []} in
+    let eeb = log @@ EncryptedExtensions(ee) in
+    match Cert.lookup_server_chain cfg.cert_chain_file cfg.private_key_file n.n_protocol_version n.n_sigAlg n.n_extensions.ne_signature_algorithms with
+    | Correct (chain, csk) -> 
+      let c = {crt_chain = chain} in
+      let cb = log @@ Certificate(c) in
+      let cr = n.n_client_random in
+      let ems = n.n_extensions.ne_extended_ms in
+      let pv = n.n_protocol_version in 
+      let cs = n.n_cipher_suite in
+
+      let sv = HandshakeLog.getBytes(log) in
+      let finv = HandshakeLog.getHash(log) in
+
+      // Signature agility (following the broken rules of 7.4.1.4.1. in RFC5246)
+      let Some sa = n.n_sigAlg in
+      let algs = match n.n_extensions.ne_signature_algorithms with
+        | None -> [sa,Hash CoreCrypto.SHA256] | Some l -> l in
+      let algs = List.Tot.filter (fun (s,_)->s=sa) algs in
+      let alg = match algs with | h::_ -> h | [] -> (sa, Hash CoreCrypto.SHA256) in
+
+      (match Cert.sign pv Server (None) csk alg sv with
+      | Correct signature -> 
+         let scv = {cv_sig = signature} in
+         let scvb = log @@ CertificateVerify(scv) in
+	 let svd = KeySchedule.ks_server_13_server_finished ks finv in
+	 let fin = {fin_vd = svd} in
+	 let finb = log @@ Finished(fin) in
+	 Correct [(EncryptedExtensions(ee),eeb);(Certificate(c),cb);(CertificateVerify(scv),scvb);(Finished(fin),finb)]
+      | Error z -> Error z)
+    | Error z -> Error z
+    else 
+       Error (AD_handshake_failure, perror __SOURCE_FILE__ __LINE__ "should not call this function in TLS < 1.3")
+
+val server_send_server_finished_13: hs -> ST unit
   (requires (fun h -> True))
   (ensures (fun h0 i h1 -> True))
+let server_send_server_finished_13 (HS #r0 r res cfg id lgref hsref) =
+  match (!hsref).hs_state with
+  | S(S_HelloSent n) 
+    when (n.n_protocol_version = TLS_1p3 &&
+	 (n.n_kexAlg = Kex_DHE || n.n_kexAlg = Kex_ECDHE)) ->
+    (match prepareServerFinished_13 cfg n (!hsref).hs_ks (!hsref).hs_log with
+     | Correct ([(EncryptedExtensions(ee),eeb);(Certificate(c),cb);(CertificateVerify(scv),scvb);(Finished(f),sfinb)]) ->    
+            let nl = eeb @| cb @| scvb @| sfinb in
+	    hsref := {!hsref with
+		 hs_buffers = {(!hsref).hs_buffers with hs_outgoing = nl};
+		 hs_state = S(S_FinishedSent n)}
+     | Error e -> 
+	  hsref := {!hsref with hs_state = S(S_Error e)})
+
+
+val processClientFinished_13: KeySchedule.ks -> HandshakeLog.log -> list (hs_msg * bytes) -> list (hs_msg * bytes) ->
+    			      ST (result (bytes * KeySchedule.recordInstance))
+  (requires (fun h -> True))
+  (ensures (fun h0 i h1 -> True))
+let processClientFinished_13 ks log msgs opt_msgs =
+   let rem = 
+   match opt_msgs with
+   | [(Certificate c,_)] ->
+     let _ = log @@ Certificate(c) in
+     Correct msgs
+   | [] -> Correct msgs 
+   | _ -> Error(AD_decode_error, perror __SOURCE_FILE__ __LINE__ "Expected Certificate only before CKE") in
+   match rem with
+   | Correct ([(Finished(f),finb)]) ->
+     let lb = HandshakeLog.getHash log in
+     let (cvd,keys) = KeySchedule.ks_server_13_client_finished ks lb in
+     if (equalBytes cvd f.fin_vd) then 
+     	let _ = log @@ (Finished(f)) in
+	Correct (cvd,keys)
+     else Error (AD_decode_error, "Finished MAC did not verify")
+   | _ -> Error (AD_decode_error, "Unexpected state")
+
+
+val server_handle_client_finished_13: hs -> list (hs_msg * bytes) -> list (hs_msg * bytes) -> ST incoming
+  (requires (fun h -> True))
+  (ensures (fun h0 i h1 -> True))
+let server_handle_client_finished_13 (HS #r0 r res cfg id lgref hsref) msgs opt_msgs =
+  match (!hsref).hs_state with
+  | S(S_FinishedSent n) -> 
+    (match processClientFinished_13 (!hsref).hs_ks (!hsref).hs_log msgs opt_msgs with
+     | Correct svd ->
+       (hsref := {!hsref with
+  	           hs_state = S(S_Idle None)};
+        InAck false false)
+     | Error z -> InError z)
+
+
+(* TODO: resumption *)
 assume val server_send_server_finished_res: hs -> ST unit
   (requires (fun h -> True))
   (ensures (fun h0 i h1 -> True))
 
 
 
+
 (* Handshake API: PUBLIC Functions, taken from FSTI *)
 
 //val version: see .fsti
+
+
+// returns the protocol version negotiated so far
+// (used for formatting outgoing packets, but not trusted)
+val version: s:hs -> ST protocolVersion
+  (requires (hs_inv s))
+  (ensures (fun h0 pv h1 -> h0 = h1))
 let version (HS r res cfg id l st) =
     match (!st).hs_nego with
     | Some n -> n.n_protocol_version
@@ -622,7 +1114,22 @@ let iT_old (HS r res cfg id l st) rw =
   | Reader -> (!st).hs_reader
   | Writer -> (!st).hs_writer
 
+
+(*** Control Interface ***)
+
 //val init: see .fsti
+// Create instance for a fresh connection, with optional resumption for clients
+val init: r0:rid -> r: role -> cfg:config -> resume: resume_id r -> 
+  ST hs
+  (requires (fun h -> True))
+  (ensures (fun h0 s h1 ->
+    modifies Set.empty h0 h1 /\
+    fresh_subregion r0 (HS.region s) h0 h1 /\
+    hs_inv s h1 /\
+    HS.r s = r /\
+    HS.resume s = resume /\
+    HS.cfg s = cfg /\
+    logT s h1 = Seq.createEmpty ))
 let init r0 r cfg res = 
     let id = Nonce.mkHelloRandom r r0 in //NS: should this really be Client?
     let lgref = MS.alloc_mref_seq r0 Seq.createEmpty in
@@ -630,19 +1137,63 @@ let init r0 r cfg res =
     let hsref = ralloc r0 hs in
     HS #r0 r res cfg id lgref hsref
 
+let mods s h0 h1 = 
+  HyperHeap.modifies_one s.region h0 h1
+  
+let modifies_internal h0 s h1 =
+    hs_inv s h1 /\
+    mods s h0 h1 /\ 
+    modifies_rref s.region !{as_ref s.state} h0 h1
+
 // Idle client starts a full handshake on the current connection
+val rehandshake: s:hs -> config -> ST bool
+  (requires (fun h -> hs_inv s h /\ HS.r s = Client))
+  (ensures (fun h0 _ h1 -> modifies_internal h0 s h1))
 let rehandshake s c = Platform.Error.unexpected "rehandshake: not yet implemented"
 
 // Idle client starts an abbreviated handshake resuming the current session
+val rekey: s:hs -> config -> ST bool
+  (requires (fun h -> hs_inv s h /\ HS.r s = Client))
+  (ensures (fun h0 _ h1 -> modifies_internal h0 s h1))
 let rekey s c = Platform.Error.unexpected "rekey: not yet implemented"
 
 // (Idle) Server requests an handshake
+val request: s:hs -> config -> ST bool
+  (requires (fun h -> hs_inv s h /\ HS.r s = Server))
+  (ensures (fun h0 _ h1 -> modifies_internal h0 s h1))
 let request s c = Platform.Error.unexpected "request: not yet implemented"
 
+val invalidateSession: s:hs -> ST unit
+  (requires (hs_inv s))
+  (ensures (fun h0 _ h1 -> modifies_internal h0 s h1)) // underspecified
 let invalidateSession hs = Platform.Error.unexpected "invalidateSession: not yet implemented"
 
+
+(*** Outgoing (main) ***)
+
 //val next_fragment: see .fsti
-let rec next_fragment hs = 
+let next_fragment_ensures (#i:id) (s:hs) h0 (result:outgoing i) h1 = 
+    let es = logT s h0 in
+    let w0 = iT s Writer h0 in
+    let w1 = iT s Writer h1 in
+    let r0 = iT s Reader h0 in
+    let r1 = iT s Reader h1 in
+    hs_inv s h1 /\
+    mods s h0 h1 /\
+    r1 == r0 /\
+//  w1 == (match result with | Outgoing _ _ true _ -> w0 + 1 | _ -> w0 ) /\
+    w1 == (if out_next_keys result then  w0 + 1 else w0 ) /\
+    (b2t (out_complete result) ==> w1 >= 0 /\ r1 = w1 /\ iT s Writer h1 >= 0 /\ completed (eT s Writer h1)) 
+
+val next_fragment: i:id -> s:hs -> ST (outgoing i)
+  (requires (fun h0 -> 
+    let es = logT s h0 in
+    let j = iT s Writer h0 in 
+    hs_inv s h0 /\
+    (if j = -1 then i = noId else let e = Seq.index es j in i = hsId e.h)   
+  ))
+  (ensures (next_fragment_ensures s))
+let rec next_fragment i hs = 
     let (HS #r0 r res cfg id lgref hsref) = hs in
     let pv,kex,res = 
       (match (!hsref).hs_nego with 
@@ -652,20 +1203,22 @@ let rec next_fragment hs =
     let l = length b in
     if (l > 0) then (
        hsref := {!hsref with hs_buffers = {(!hsref).hs_buffers with hs_outgoing = empty_bytes}};
-       OutSome (l,l) b) 
+       Outgoing (Some (out_msg i (l,l) b)) false false false)
     else 
       (match (!hsref).hs_state with 
        | C (C_Error e) -> OutError e
        | S (S_Error e) -> OutError e
-       | C (C_Idle ri) -> (client_send_client_hello hs; next_fragment hs)
-       | C (C_OutCCS n) -> (client_send_client_finished hs; OutCCS)
-       | S (S_HelloSent n) when (is_Some pv && pv <> Some TLS_1p3 && res = Some false) -> server_send_server_hello_done hs; next_fragment hs
-       | S (S_HelloSent n) when (is_Some pv && pv <> Some TLS_1p3 && res = Some true) -> server_send_server_finished_res hs; next_fragment hs
-       | S (S_HelloSent n) when (is_Some pv && pv = Some TLS_1p3) -> server_send_server_finished_13 hs; next_fragment hs
-       | S (S_OutCCS s) -> server_send_server_finished hs; OutCCS)
+       | C (C_Idle ri) -> (client_send_client_hello hs; next_fragment i hs)
+       | C (C_OutCCS n) -> (client_send_client_finished hs; Outgoing None true true false)
+       | S (S_HelloSent n) when (is_Some pv && pv <> Some TLS_1p3 && res = Some false) -> server_send_server_hello_done hs; next_fragment i hs
+       | S (S_HelloSent n) when (is_Some pv && pv <> Some TLS_1p3 && res = Some true) -> server_send_server_finished_res hs; next_fragment i hs
+       | S (S_HelloSent n) when (is_Some pv && pv = Some TLS_1p3) -> server_send_server_finished_13 hs; next_fragment i hs
+       | S (S_OutCCS n) -> server_send_server_finished hs; Outgoing None true true false)
 
 
+(*** Incoming (main) ***)
 
+val parseHandshakeMessages : option protocolVersion -> option kexAlg -> buf:bytes -> Tot  (result (rem:bytes * list (hs_msg * bytes)))
 let rec parseHandshakeMessages pv kex buf =
     match parseMessage buf with
     | Error z -> Error z
@@ -679,8 +1232,22 @@ let rec parseHandshakeMessages pv kex buf =
        	     | Correct (r,hsl) -> Correct(r,(hsm,to_log)::hsl)))
 
 
-//val recv_fragment: see .fsti
-let recv_fragment hs (rg:Range.range) (rb:rbytes rg) = 
+let recv_ensures (s:hs) (h0:HyperHeap.t) (result:incoming) (h1:HyperHeap.t) = 
+    let w0 = iT s Writer h0 in
+    let w1 = iT s Writer h1 in
+    let r0 = iT s Reader h0 in
+    let r1 = iT s Reader h1 in
+    hs_inv s h1 /\
+    mods s h0 h1 /\
+    w1 == w0 /\
+    r1 == (if in_next_keys result then r0 + 1 else r0) /\
+    (b2t (in_complete result) ==> r1 >= 0 /\ r1 = w1 /\ iT s Reader h1 >= 0 /\ completed (eT s Reader h1))
+
+val recv_fragment: s:hs -> #i:id -> message i -> ST incoming
+  (requires (hs_inv s))
+  (ensures (recv_ensures s))
+let recv_fragment hs #i f = 
+    let (| rg,rb |) = f in
     let (HS #r0 r res cfg id lgref hsref) = hs in
     let b = (!hsref).hs_buffers.hs_incoming in
     let b = b @| rb in
@@ -723,7 +1290,6 @@ let recv_fragment hs (rg:Range.range) (rb:rbytes rg) =
 			   (ServerKeyExchange(ske),l') ;
 			   (ServerHelloDone,l''')] 
 			   [(CertificateRequest(cr),l'')]
-
        
        | C (C_CCSReceived n cv), (Finished(f),l)::hsl 
        	 when (is_Some pv && pv <> Some TLS_1p3) ->
@@ -759,7 +1325,6 @@ let recv_fragment hs (rg:Range.range) (rb:rbytes rg) =
 			   (Certificate(c),l2) ;			   
 			   (CertificateVerify(cv),l3) ;
 			   (Finished(f),l4)]
-			   
        
        | S (S_Idle ri), (ClientHello(ch),l)::hsl -> 
 	   hsref := {!hsref with hs_buffers = {(!hsref).hs_buffers with hs_incoming_parsed = hsl}};
@@ -794,10 +1359,15 @@ let recv_fragment hs (rg:Range.range) (rb:rbytes rg) =
 
        | C (C_Error e),_ -> InError e
        | S (S_Error e),_ -> InError e
-       | _ , _ -> InAck)
+       | _ , _ -> InAck false false)
 	   
 
-//val recv_ccs: see .fsti  // special case: CCS before 1p3  
+val recv_ccs: s:hs -> ST incoming  // special case: CCS before 1p3; could merge with recv_fragment
+  (requires (hs_inv s)) // could require pv <= 1p2
+  (ensures (fun h0 result h1 ->
+    recv_ensures s h0 result h1 /\
+    (is_InError result \/ result = InAck true false)
+    ))
 let recv_ccs hs = 
     let (HS #r0 r res cfg id lgref hsref) = hs in
     let pv,kex = 
@@ -839,4 +1409,8 @@ let recv_ccs hs =
     | _,_ -> InError(AD_unexpected_message, "ClientCCS received at wrong time"))
 
 
+val authorize: s:hs -> Cert.chain -> ST incoming // special case: explicit authorize (needed?)
+  (requires (hs_inv s))
+  (ensures (fun h0 result h1 ->
+    (is_InAck result \/ is_InError result) /\ recv_ensures s h0 result h1 ))
 let authorize s ch = Platform.Error.unexpected "authorize: not yet implemented"
