src/tls/Connection.fst
@@ -18,7 +18,7 @@ open TLSInfo
   
 open Range
 
-open MergedHandshake module Handshake = MergedHandshake //16-05-20 open Handshake
+open Handshake
 
 module MR = FStar.Monotonic.RRef
 
